Setlec.lean
@@ -14,5 +14,6 @@ import Setlec.Model.Interp
 import Setlec.Model.InterpLemmas
 import Setlec.Model.TypeChecker
 import Setlec.Model.IndInstall
+import Setlec.Model.ProjInstall
 import Setlec.Model.Extend
 import Setlec.Model.Consistency
